meta-theory/pure_barendregtScript.sml
@@ -1,0 +1,218 @@
+(*
+  Barendregt convention for PureLang
+*)
+open HolKernel Parse boolLib bossLib BasicProvers dep_rewrite;
+open pairTheory listTheory rich_listTheory pred_setTheory;
+
+open pure_expTheory pure_exp_lemmasTheory pure_miscTheory pure_beta_equivTheory;
+
+val _ = new_theory "pure_barendregt";
+
+
+(********** Preliminaries: lists of pairwise-disjoint sets *)
+
+Definition list_disjoint_def:
+  list_disjoint l ⇔
+    ∀left mid right.
+      l = left ++ [mid] ++ right
+    ⇒ DISJOINT mid (BIGUNION (set (left ++ right)))
+End
+
+Theorem list_disjoint_alt_def:
+  list_disjoint l ⇔
+    ∀left right. l = left ++ right ⇒
+      DISJOINT (BIGUNION (set left)) (BIGUNION (set right))
+Proof
+  rw[list_disjoint_def] >> eq_tac >> rw[]
+  >- (
+    first_x_assum irule >>
+    qspecl_then [`left`,`s'`] assume_tac $ GEN_ALL MEM_SING_APPEND >> gvs[] >>
+    qexists_tac `a` >> simp[]
+    )
+  >- (
+    once_rewrite_tac[DISJOINT_SYM] >>
+    first_x_assum irule >> qexists_tac `left` >> simp[]
+    )
+  >- (first_x_assum irule >> qexists_tac `left ++ [mid]` >> simp[])
+QED
+
+Theorem list_disjoint_cons:
+  list_disjoint (x::xs) ⇔
+    list_disjoint xs ∧ EVERY (DISJOINT x) xs
+Proof
+  rw[list_disjoint_alt_def] >> eq_tac >> rw[]
+  >- (first_x_assum irule >> qexists `x::left` >> simp[])
+  >- (
+    first_x_assum $ qspec_then `[x]` assume_tac >> gvs[EVERY_MEM]
+    ) >>
+  gvs[APPEND_EQ_CONS, EVERY_MEM] >>
+  first_x_assum irule >> rpt $ goal_assum $ drule_at Any >> simp[]
+QED
+
+Theorem list_disjoint_singleton[simp]:
+  list_disjoint [a]
+Proof
+  rw[list_disjoint_alt_def] >> Cases_on `left` >> gvs[]
+QED
+
+Theorem list_disjoint_doubleton[simp]:
+  list_disjoint [a;b] ⇔ DISJOINT a b
+Proof
+  rw[list_disjoint_def] >> eq_tac >> rw[]
+  >- (first_x_assum irule >> qexistsl_tac [`[]`] >> simp[]) >>
+  Cases_on `left` >> gvs[] >> Cases_on `t` >> gvs[] >> simp[DISJOINT_SYM]
+QED
+
+Theorem list_disjoint_append:
+  ∀l1 l2. list_disjoint (l1 ++ l2) ⇔
+    list_disjoint l1 ∧ list_disjoint l2 ∧
+    DISJOINT (BIGUNION (set l1)) (BIGUNION (set l2))
+Proof
+  rw[list_disjoint_alt_def] >> eq_tac >> rw[]
+  >- (first_x_assum irule >> qexists_tac `left` >> simp[])
+  >- (first_x_assum irule >> qexists_tac `l1 ++ left` >> simp[])
+  >- (first_x_assum irule >> qexists_tac `l1` >> simp[]) >>
+  gvs[APPEND_EQ_APPEND]
+  >- (last_x_assum irule >> ntac 2 $ goal_assum drule >> simp[])
+  >- (
+    last_x_assum kall_tac >> last_x_assum irule >>
+    ntac 2 $ goal_assum drule >> simp[]
+    )
+QED
+
+Theorem list_disjoint_ALL_DISTINCT:
+  ∀l. EVERY FINITE l ⇒
+    (list_disjoint l ⇔ ALL_DISTINCT (FLAT $ MAP SET_TO_LIST l))
+Proof
+  Induct >- rw[list_disjoint_def] >>
+  rw[list_disjoint_cons, ALL_DISTINCT_APPEND] >> gvs[] >>
+  irule AND_CONG >> rw[] >> eq_tac >> rw[]
+  >- (
+    CCONTR_TAC >> gvs[] >>
+    gvs[MEM_FLAT, MEM_MAP, EVERY_MEM, MEM_SET_TO_LIST, DISJOINT_ALT]
+    )
+  >- (
+    gvs[Once MONO_NOT_EQ] >>
+    gvs[MEM_FLAT, MEM_MAP, PULL_EXISTS, EVERY_MEM] >> rw[] >>
+    first_x_assum drule >> gvs[MEM_SET_TO_LIST, DISJOINT_ALT] >> metis_tac[]
+    )
+QED
+
+
+(********** Unique bound variables **********)
+
+Definition unique_boundvars_def:
+  unique_boundvars (Var x) = T ∧
+  unique_boundvars (Prim op es) =
+    (EVERY unique_boundvars es ∧ list_disjoint (MAP boundvars es)) ∧
+  unique_boundvars (App e1 e2) = (
+    unique_boundvars e1 ∧ unique_boundvars e2 ∧
+    DISJOINT (boundvars e1) (boundvars e2)) ∧
+  unique_boundvars (Lam x e) = (x ∉ boundvars e ∧ unique_boundvars e) ∧
+  unique_boundvars (Letrec fns e) = (
+    ALL_DISTINCT (MAP FST fns) ∧
+    list_disjoint (set (MAP FST fns) :: MAP boundvars (e::MAP SND fns)) ∧
+    EVERY unique_boundvars (e :: MAP SND fns))
+Termination
+  WF_REL_TAC `measure exp_size` >>
+  Induct >> rw[] >> gvs[SF DNF_ss] >>
+  PairCases_on `h` >> gvs[pure_expTheory.exp_size_def] >>
+  first_x_assum drule >> disch_then $ qspec_then `e` assume_tac >> gvs[]
+End
+
+Theorem unique_boundvars_Letrec:
+  unique_boundvars (Letrec fns e) ⇔
+    ALL_DISTINCT (MAP FST fns) ∧
+    let names = set $ MAP FST fns in
+      EVERY (λ(f,body).
+        DISJOINT names (boundvars body) ∧
+        DISJOINT (boundvars e) (boundvars body) ∧
+        unique_boundvars body) fns ∧
+      list_disjoint (MAP boundvars (MAP SND fns)) ∧
+      DISJOINT names (boundvars e) ∧
+      unique_boundvars e
+Proof
+  rw[unique_boundvars_def] >> irule_at Any AND_CONG >> rw[] >>
+  simp[list_disjoint_cons] >> eq_tac >> rw[] >>
+  gvs[EVERY_MEM, MEM_MAP, EXISTS_PROD] >> gvs[PULL_EXISTS] >> rw[]
+  >- (pairarg_tac >> gvs[] >> rpt $ last_assum $ irule_at Any) >>
+  first_x_assum drule >> gvs[]
+QED
+
+Theorem unique_boundvars_thm:
+  ∀e. unique_boundvars e ⇔ ALL_DISTINCT (boundvars_l e)
+Proof
+  Induct using unique_boundvars_ind >>
+  rw[unique_boundvars_Letrec, unique_boundvars_def] >>
+  gvs[ALL_DISTINCT_APPEND]
+  >- (
+    Induct_on `es` >> rw[] >> gvs[] >- simp[list_disjoint_def] >>
+    gvs[list_disjoint_cons, ALL_DISTINCT_APPEND] >>
+    gvs[EVERY_MEM, MEM_MAP, MEM_FLAT, DISJOINT_ALT, boundvars_equiv, PULL_EXISTS] >>
+    metis_tac[]
+    )
+  >- gvs[DISJOINT_ALT, boundvars_equiv]
+  >- gvs[boundvars_equiv] >>
+  eq_tac >> strip_tac
+  >- (
+    gvs[SF DNF_ss, EVERY_MEM, DISJOINT_ALT, boundvars_equiv,
+        MEM_FLAT, MEM_MAP, PULL_EXISTS, FORALL_PROD] >>
+    reverse $ rw[] >- metis_tac[] >- metis_tac[] >- metis_tac[] >>
+    `∀f body. MEM (f,body) fns ⇒ ALL_DISTINCT (boundvars_l body)` by metis_tac[] >>
+    pop_assum mp_tac >> qpat_x_assum `list_disjoint _` mp_tac >>
+    rpt $ pop_assum kall_tac >> Induct_on `fns` >> rw[] >> gvs[SF DNF_ss] >>
+    pairarg_tac >> gvs[ALL_DISTINCT_APPEND, list_disjoint_cons] >>
+    first_x_assum $ irule_at Any >> conj_tac >> gvs[] >>
+    gvs[MAP_MAP_o, combinTheory.o_DEF, LAMBDA_PROD] >>
+    gvs[MEM_FLAT, MEM_MAP, EVERY_MEM, DISJOINT_ALT,
+        EXISTS_PROD, FORALL_PROD, boundvars_equiv] >>
+    metis_tac[]
+    )
+  >- (
+    gvs[SF DNF_ss, EVERY_MEM, DISJOINT_ALT, boundvars_equiv,
+        MEM_FLAT, MEM_MAP, PULL_EXISTS, FORALL_PROD] >>
+    rw[] >- metis_tac[] >- metis_tac[]
+    >~ [`¬MEM x (boundvars_l e)`] >- metis_tac[]
+    >- (
+      drule ALL_DISTINCT_FLAT_IMP >> simp[MEM_MAP, PULL_EXISTS] >>
+      disch_then drule >> simp[] >> metis_tac[]
+      ) >>
+    DEP_REWRITE_TAC[list_disjoint_ALL_DISTINCT] >> simp[EVERY_MAP] >>
+    simp[MAP_MAP_o, combinTheory.o_DEF, LAMBDA_PROD] >>
+    qpat_x_assum `ALL_DISTINCT (FLAT _)` mp_tac >> rpt $ pop_assum kall_tac >>
+    Induct_on `fns` >> rw[] >> gvs[] >> pairarg_tac >> gvs[] >>
+    gvs[ALL_DISTINCT_APPEND, boundvars_equiv] >> rw[] >>
+    first_x_assum drule >> simp[MEM_FLAT, MEM_MAP, FORALL_PROD] >>
+    rw[DISJ_EQ_IMP, PULL_FORALL, PULL_EXISTS] >> res_tac
+    )
+QED
+
+
+(********** Barendregt convention **********)
+
+Definition barendregt_def:
+  barendregt e ⇔ unique_boundvars e ∧ DISJOINT (boundvars e) (freevars e)
+End
+
+Theorem barendregt_beta_equivalence:
+  barendregt (App (Lam x body) arg) ⇒
+    App (Lam x body) arg ≅ subst1 x arg body
+Proof
+  rw[barendregt_def] >> irule disjoint_vars_beta_equivalence >> simp[]
+QED
+
+Theorem barendregt_beta_equivalence_Letrec:
+  barendregt (Letrec fns e) ⇒
+    Letrec fns e ≅ subst (FEMPTY |++ (MAP (λ(f,body). f, Letrec fns body) fns)) e
+Proof
+  rw[barendregt_def] >>
+  irule disjoint_vars_beta_equivalence_Letrec >> rw[EVERY_MEM] >>
+  pairarg_tac >> gvs[] >> simp[Once DISJOINT_SYM] >> gvs[DISJOINT_ALT] >> rw[] >>
+  last_x_assum drule >> strip_tac >>
+  gvs[DISJ_EQ_IMP, MEM_MAP, PULL_EXISTS, EXISTS_PROD] >> metis_tac[]
+QED
+
+
+(**********)
+
+val _ = export_theory();
